coq/ZF/Meta/Term/HasTyDecl.v
@@ -4,7 +4,7 @@ Require Import ZF.Meta.Term.HasTy.
 
 (* A term declaration is well typed when its body has its declared sort.        *)
 Definition HasTyDecl (e:Env) (d:Decl) : Prop :=
-  match Term.Decl.body d with
-  | Some t => HasTy e (Term.Decl.ctx d) t (Term.Decl.res d)
+  match bodyT d with
+  | Some t => HasTy e (ctxT d) t (resT d)
   | None   => True
   end.
